tests/lean/hashmap/Hashmap/Funs.lean
@@ -5,19 +5,19 @@ import Hashmap.Types
 import Hashmap.Clauses.Clauses
 
 /- [hashmap::hash_key] -/
-def hash_key_fwd (k : USize) : Result USize :=
+def hash_key_fwd (k : Usize) : Result Usize :=
   Result.ret k
 
 /- [hashmap::HashMap::{0}::allocate_slots] -/
 def hash_map_allocate_slots_loop_fwd
-  (T : Type) (slots : Vec (list_t T)) (n : USize) :
+  (T : Type) (slots : Vec (list_t T)) (n : Usize) :
   (Result (Vec (list_t T)))
   :=
-  if 𝒽: n > (USize.ofNatCore 0 (by intlit))
+  if 𝒽: n > (Usize.ofInt 0 (by intlit))
   then
     do
-      let slots0 ⟵ vec_push_back (list_t T) slots list_t.ListNil
-      let n0 ⟵ USize.checked_sub n (USize.ofNatCore 1 (by intlit))
+      let slots0 ⟵ vec_push_back (list_t T) slots list_t.Nil
+      let n0 ⟵ n - (Usize.ofInt 1 (by intlit))
       let v ⟵ hash_map_allocate_slots_loop_fwd T slots0 n0
       Result.ret v
   else Result.ret slots
@@ -27,25 +27,25 @@ decreasing_by hash_map_allocate_slots_loop_decreases slots n
 
 /- [hashmap::HashMap::{0}::allocate_slots] -/
 def hash_map_allocate_slots_fwd
-  (T : Type) (slots : Vec (list_t T)) (n : USize) : Result (Vec (list_t T)) :=
+  (T : Type) (slots : Vec (list_t T)) (n : Usize) : Result (Vec (list_t T)) :=
   do
     let v ⟵ hash_map_allocate_slots_loop_fwd T slots n
     Result.ret v
 
 /- [hashmap::HashMap::{0}::new_with_capacity] -/
 def hash_map_new_with_capacity_fwd
-  (T : Type) (capacity : USize) (max_load_dividend : USize)
-  (max_load_divisor : USize) :
+  (T : Type) (capacity : Usize) (max_load_dividend : Usize)
+  (max_load_divisor : Usize) :
   Result (hash_map_t T)
   :=
   do
     let v := vec_new (list_t T)
     let slots ⟵ hash_map_allocate_slots_fwd T v capacity
-    let i ⟵ USize.checked_mul capacity max_load_dividend
-    let i0 ⟵ USize.checked_div i max_load_divisor
+    let i ⟵ capacity * max_load_dividend
+    let i0 ⟵ i / max_load_divisor
     Result.ret
       {
-        hash_map_num_entries := (USize.ofNatCore 0 (by intlit)),
+        hash_map_num_entries := (Usize.ofInt 0 (by intlit)),
         hash_map_max_load_factor := (max_load_dividend, max_load_divisor),
         hash_map_max_load := i0,
         hash_map_slots := slots
@@ -53,135 +53,128 @@ def hash_map_new_with_capacity_fwd
 
 /- [hashmap::HashMap::{0}::new] -/
 def hash_map_new_fwd (T : Type) : Result (hash_map_t T) :=
-  hash_map_new_with_capacity_fwd T (USize.ofNatCore 32 (by intlit))
-    (USize.ofNatCore 4 (by intlit)) (USize.ofNatCore 5 (by intlit))
+  hash_map_new_with_capacity_fwd T (Usize.ofInt 32 (by intlit))
+    (Usize.ofInt 4 (by intlit)) (Usize.ofInt 5 (by intlit))
 
-/- [hashmap::HashMap::{0}::clear] -/
-def hash_map_clear_loop_fwd_back
-  (T : Type) (slots : Vec (list_t T)) (i : USize) :
+/- [hashmap::HashMap::{0}::clear_slots] -/
+def hash_map_clear_slots_loop_fwd_back
+  (T : Type) (slots : Vec (list_t T)) (i : Usize) :
   (Result (Vec (list_t T)))
   :=
   let i0 := vec_len (list_t T) slots
   if 𝒽: i < i0
   then
     do
-      let i1 ⟵ USize.checked_add i (USize.ofNatCore 1 (by intlit))
-      let slots0 ⟵ vec_index_mut_back (list_t T) slots i list_t.ListNil
-      let v ⟵ hash_map_clear_loop_fwd_back T slots0 i1
+      let i1 ⟵ i + (Usize.ofInt 1 (by intlit))
+      let slots0 ⟵ vec_index_mut_back (list_t T) slots i list_t.Nil
+      let v ⟵ hash_map_clear_slots_loop_fwd_back T slots0 i1
       Result.ret v
   else Result.ret slots
-termination_by hash_map_clear_loop_fwd_back slots i =>
-  hash_map_clear_loop_terminates T slots i
-decreasing_by hash_map_clear_loop_decreases slots i
+termination_by hash_map_clear_slots_loop_fwd_back slots i =>
+  hash_map_clear_slots_loop_terminates T slots i
+decreasing_by hash_map_clear_slots_loop_decreases slots i
+
+/- [hashmap::HashMap::{0}::clear_slots] -/
+def hash_map_clear_slots_fwd_back
+  (T : Type) (slots : Vec (list_t T)) : Result (Vec (list_t T)) :=
+  do
+    let v ⟵
+      hash_map_clear_slots_loop_fwd_back T slots (Usize.ofInt 0 (by intlit))
+    Result.ret v
 
 /- [hashmap::HashMap::{0}::clear] -/
 def hash_map_clear_fwd_back
   (T : Type) (self : hash_map_t T) : Result (hash_map_t T) :=
   do
-    let v ⟵
-      hash_map_clear_loop_fwd_back T self.hash_map_slots
-        (USize.ofNatCore 0 (by intlit))
+    let v ⟵ hash_map_clear_slots_fwd_back T self.hash_map_slots
     Result.ret
       {
-        hash_map_num_entries := (USize.ofNatCore 0 (by intlit)),
-        hash_map_max_load_factor := self.hash_map_max_load_factor,
-        hash_map_max_load := self.hash_map_max_load,
-        hash_map_slots := v
+        self
+          with
+          hash_map_num_entries := (Usize.ofInt 0 (by intlit)),
+          hash_map_slots := v
       }
 
 /- [hashmap::HashMap::{0}::len] -/
-def hash_map_len_fwd (T : Type) (self : hash_map_t T) : Result USize :=
+def hash_map_len_fwd (T : Type) (self : hash_map_t T) : Result Usize :=
   Result.ret self.hash_map_num_entries
 
 /- [hashmap::HashMap::{0}::insert_in_list] -/
 def hash_map_insert_in_list_loop_fwd
-  (T : Type) (key : USize) (value : T) (ls : list_t T) : (Result Bool) :=
+  (T : Type) (key : Usize) (value : T) (ls : list_t T) : (Result Bool) :=
   match 𝒽: ls with
-  | list_t.ListCons ckey cvalue tl =>
+  | list_t.Cons ckey cvalue tl =>
     if 𝒽: ckey = key
     then Result.ret false
     else
       do
         let b ⟵ hash_map_insert_in_list_loop_fwd T key value tl
         Result.ret b
-  | list_t.ListNil => Result.ret true
+  | list_t.Nil => Result.ret true
 termination_by hash_map_insert_in_list_loop_fwd key value ls =>
   hash_map_insert_in_list_loop_terminates T key value ls
 decreasing_by hash_map_insert_in_list_loop_decreases key value ls
 
 /- [hashmap::HashMap::{0}::insert_in_list] -/
 def hash_map_insert_in_list_fwd
-  (T : Type) (key : USize) (value : T) (ls : list_t T) : Result Bool :=
+  (T : Type) (key : Usize) (value : T) (ls : list_t T) : Result Bool :=
   do
     let b ⟵ hash_map_insert_in_list_loop_fwd T key value ls
     Result.ret b
 
 /- [hashmap::HashMap::{0}::insert_in_list] -/
 def hash_map_insert_in_list_loop_back
-  (T : Type) (key : USize) (value : T) (ls : list_t T) : (Result (list_t T)) :=
+  (T : Type) (key : Usize) (value : T) (ls : list_t T) : (Result (list_t T)) :=
   match 𝒽: ls with
-  | list_t.ListCons ckey cvalue tl =>
+  | list_t.Cons ckey cvalue tl =>
     if 𝒽: ckey = key
-    then Result.ret (list_t.ListCons ckey value tl)
+    then Result.ret (list_t.Cons ckey value tl)
     else
       do
         let tl0 ⟵ hash_map_insert_in_list_loop_back T key value tl
-        Result.ret (list_t.ListCons ckey cvalue tl0)
-  | list_t.ListNil =>
-    let l := list_t.ListNil
-    Result.ret (list_t.ListCons key value l)
+        Result.ret (list_t.Cons ckey cvalue tl0)
+  | list_t.Nil => let l := list_t.Nil
+                  Result.ret (list_t.Cons key value l)
 termination_by hash_map_insert_in_list_loop_back key value ls =>
   hash_map_insert_in_list_loop_terminates T key value ls
 decreasing_by hash_map_insert_in_list_loop_decreases key value ls
 
 /- [hashmap::HashMap::{0}::insert_in_list] -/
 def hash_map_insert_in_list_back
-  (T : Type) (key : USize) (value : T) (ls : list_t T) : Result (list_t T) :=
+  (T : Type) (key : Usize) (value : T) (ls : list_t T) : Result (list_t T) :=
   do
     let l ⟵ hash_map_insert_in_list_loop_back T key value ls
     Result.ret l
 
 /- [hashmap::HashMap::{0}::insert_no_resize] -/
 def hash_map_insert_no_resize_fwd_back
-  (T : Type) (self : hash_map_t T) (key : USize) (value : T) :
+  (T : Type) (self : hash_map_t T) (key : Usize) (value : T) :
   Result (hash_map_t T)
   :=
   do
     let hash ⟵ hash_key_fwd key
     let i := vec_len (list_t T) self.hash_map_slots
-    let hash_mod ⟵ USize.checked_rem hash i
+    let hash_mod ⟵ hash % i
     let l ⟵ vec_index_mut_fwd (list_t T) self.hash_map_slots hash_mod
     let inserted ⟵ hash_map_insert_in_list_fwd T key value l
     if 𝒽: inserted
     then
       do
-        let i0 ⟵ USize.checked_add self.hash_map_num_entries
-          (USize.ofNatCore 1 (by intlit))
+        let i0 ⟵ self.hash_map_num_entries + (Usize.ofInt 1 (by intlit))
         let l0 ⟵ hash_map_insert_in_list_back T key value l
         let v ⟵ vec_index_mut_back (list_t T) self.hash_map_slots hash_mod l0
         Result.ret
-          {
-            hash_map_num_entries := i0,
-            hash_map_max_load_factor := self.hash_map_max_load_factor,
-            hash_map_max_load := self.hash_map_max_load,
-            hash_map_slots := v
-          }
+          { self with hash_map_num_entries := i0, hash_map_slots := v }
     else
       do
         let l0 ⟵ hash_map_insert_in_list_back T key value l
         let v ⟵ vec_index_mut_back (list_t T) self.hash_map_slots hash_mod l0
-        Result.ret
-          {
-            hash_map_num_entries := self.hash_map_num_entries,
-            hash_map_max_load_factor := self.hash_map_max_load_factor,
-            hash_map_max_load := self.hash_map_max_load,
-            hash_map_slots := v
-          }
+        Result.ret { self with hash_map_slots := v }
 
 /- [core::num::u32::{9}::MAX] -/
-def core_num_u32_max_body : Result UInt32 :=
-  Result.ret (UInt32.ofNatCore 4294967295 (by intlit))
-def core_num_u32_max_c : UInt32 := eval_global core_num_u32_max_body (by simp)
+def core_num_u32_max_body : Result U32 :=
+  Result.ret (U32.ofInt 4294967295 (by intlit))
+def core_num_u32_max_c : U32 := eval_global core_num_u32_max_body (by simp)
 
 /- [hashmap::HashMap::{0}::move_elements_from_list] -/
 def hash_map_move_elements_from_list_loop_fwd_back
@@ -189,12 +182,12 @@ def hash_map_move_elements_from_list_loop_fwd_back
   (Result (hash_map_t T))
   :=
   match 𝒽: ls with
-  | list_t.ListCons k v tl =>
+  | list_t.Cons k v tl =>
     do
       let ntable0 ⟵ hash_map_insert_no_resize_fwd_back T ntable k v
       let hm ⟵ hash_map_move_elements_from_list_loop_fwd_back T ntable0 tl
       Result.ret hm
-  | list_t.ListNil => Result.ret ntable
+  | list_t.Nil => Result.ret ntable
 termination_by hash_map_move_elements_from_list_loop_fwd_back ntable ls =>
   hash_map_move_elements_from_list_loop_terminates T ntable ls
 decreasing_by hash_map_move_elements_from_list_loop_decreases ntable ls
@@ -208,7 +201,7 @@ def hash_map_move_elements_from_list_fwd_back
 
 /- [hashmap::HashMap::{0}::move_elements] -/
 def hash_map_move_elements_loop_fwd_back
-  (T : Type) (ntable : hash_map_t T) (slots : Vec (list_t T)) (i : USize) :
+  (T : Type) (ntable : hash_map_t T) (slots : Vec (list_t T)) (i : Usize) :
   (Result ((hash_map_t T) × (Vec (list_t T))))
   :=
   let i0 := vec_len (list_t T) slots
@@ -216,10 +209,10 @@ def hash_map_move_elements_loop_fwd_back
   then
     do
       let l ⟵ vec_index_mut_fwd (list_t T) slots i
-      let ls := mem_replace_fwd (list_t T) l list_t.ListNil
+      let ls := mem_replace_fwd (list_t T) l list_t.Nil
       let ntable0 ⟵ hash_map_move_elements_from_list_fwd_back T ntable ls
-      let i1 ⟵ USize.checked_add i (USize.ofNatCore 1 (by intlit))
-      let l0 := mem_replace_back (list_t T) l list_t.ListNil
+      let i1 ⟵ i + (Usize.ofInt 1 (by intlit))
+      let l0 := mem_replace_back (list_t T) l list_t.Nil
       let slots0 ⟵ vec_index_mut_back (list_t T) slots i l0
       let p ⟵ hash_map_move_elements_loop_fwd_back T ntable0 slots0 i1
       let (hm, v) := p
@@ -231,7 +224,7 @@ decreasing_by hash_map_move_elements_loop_decreases ntable slots i
 
 /- [hashmap::HashMap::{0}::move_elements] -/
 def hash_map_move_elements_fwd_back
-  (T : Type) (ntable : hash_map_t T) (slots : Vec (list_t T)) (i : USize) :
+  (T : Type) (ntable : hash_map_t T) (slots : Vec (list_t T)) (i : Usize) :
   Result ((hash_map_t T) × (Vec (list_t T)))
   :=
   do
@@ -243,38 +236,31 @@ def hash_map_move_elements_fwd_back
 def hash_map_try_resize_fwd_back
   (T : Type) (self : hash_map_t T) : Result (hash_map_t T) :=
   do
-    let max_usize ⟵ scalar_cast USize core_num_u32_max_c
+    let max_usize ⟵ Scalar.cast .Usize core_num_u32_max_c
     let capacity := vec_len (list_t T) self.hash_map_slots
-    let n1 ⟵ USize.checked_div max_usize (USize.ofNatCore 2 (by intlit))
+    let n1 ⟵ max_usize / (Usize.ofInt 2 (by intlit))
     let (i, i0) := self.hash_map_max_load_factor
-    let i1 ⟵ USize.checked_div n1 i
+    let i1 ⟵ n1 / i
     if 𝒽: capacity <= i1
     then
       do
-        let i2 ⟵ USize.checked_mul capacity (USize.ofNatCore 2 (by intlit))
+        let i2 ⟵ capacity * (Usize.ofInt 2 (by intlit))
         let ntable ⟵ hash_map_new_with_capacity_fwd T i2 i i0
         let (ntable0, _) ⟵
           hash_map_move_elements_fwd_back T ntable self.hash_map_slots
-            (USize.ofNatCore 0 (by intlit))
+            (Usize.ofInt 0 (by intlit))
         Result.ret
           {
-            hash_map_num_entries := self.hash_map_num_entries,
-            hash_map_max_load_factor := (i, i0),
-            hash_map_max_load := ntable0.hash_map_max_load,
-            hash_map_slots := ntable0.hash_map_slots
+            ntable0
+              with
+              hash_map_num_entries := self.hash_map_num_entries,
+              hash_map_max_load_factor := (i, i0)
           }
-    else
-      Result.ret
-        {
-          hash_map_num_entries := self.hash_map_num_entries,
-          hash_map_max_load_factor := (i, i0),
-          hash_map_max_load := self.hash_map_max_load,
-          hash_map_slots := self.hash_map_slots
-        }
+    else Result.ret { self with hash_map_max_load_factor := (i, i0) }
 
 /- [hashmap::HashMap::{0}::insert] -/
 def hash_map_insert_fwd_back
-  (T : Type) (self : hash_map_t T) (key : USize) (value : T) :
+  (T : Type) (self : hash_map_t T) (key : Usize) (value : T) :
   Result (hash_map_t T)
   :=
   do
@@ -286,224 +272,217 @@ def hash_map_insert_fwd_back
 
 /- [hashmap::HashMap::{0}::contains_key_in_list] -/
 def hash_map_contains_key_in_list_loop_fwd
-  (T : Type) (key : USize) (ls : list_t T) : (Result Bool) :=
+  (T : Type) (key : Usize) (ls : list_t T) : (Result Bool) :=
   match 𝒽: ls with
-  | list_t.ListCons ckey t tl =>
+  | list_t.Cons ckey t tl =>
     if 𝒽: ckey = key
     then Result.ret true
     else
       do
         let b ⟵ hash_map_contains_key_in_list_loop_fwd T key tl
         Result.ret b
-  | list_t.ListNil => Result.ret false
+  | list_t.Nil => Result.ret false
 termination_by hash_map_contains_key_in_list_loop_fwd key ls =>
   hash_map_contains_key_in_list_loop_terminates T key ls
 decreasing_by hash_map_contains_key_in_list_loop_decreases key ls
 
 /- [hashmap::HashMap::{0}::contains_key_in_list] -/
 def hash_map_contains_key_in_list_fwd
-  (T : Type) (key : USize) (ls : list_t T) : Result Bool :=
+  (T : Type) (key : Usize) (ls : list_t T) : Result Bool :=
   do
     let b ⟵ hash_map_contains_key_in_list_loop_fwd T key ls
     Result.ret b
 
 /- [hashmap::HashMap::{0}::contains_key] -/
 def hash_map_contains_key_fwd
-  (T : Type) (self : hash_map_t T) (key : USize) : Result Bool :=
+  (T : Type) (self : hash_map_t T) (key : Usize) : Result Bool :=
   do
     let hash ⟵ hash_key_fwd key
     let i := vec_len (list_t T) self.hash_map_slots
-    let hash_mod ⟵ USize.checked_rem hash i
+    let hash_mod ⟵ hash % i
     let l ⟵ vec_index_fwd (list_t T) self.hash_map_slots hash_mod
     hash_map_contains_key_in_list_fwd T key l
 
 /- [hashmap::HashMap::{0}::get_in_list] -/
 def hash_map_get_in_list_loop_fwd
-  (T : Type) (key : USize) (ls : list_t T) : (Result T) :=
+  (T : Type) (key : Usize) (ls : list_t T) : (Result T) :=
   match 𝒽: ls with
-  | list_t.ListCons ckey cvalue tl =>
+  | list_t.Cons ckey cvalue tl =>
     if 𝒽: ckey = key
     then Result.ret cvalue
     else do
            let t ⟵ hash_map_get_in_list_loop_fwd T key tl
            Result.ret t
-  | list_t.ListNil => Result.fail Error.panic
+  | list_t.Nil => Result.fail Error.panic
 termination_by hash_map_get_in_list_loop_fwd key ls =>
   hash_map_get_in_list_loop_terminates T key ls
 decreasing_by hash_map_get_in_list_loop_decreases key ls
 
 /- [hashmap::HashMap::{0}::get_in_list] -/
 def hash_map_get_in_list_fwd
-  (T : Type) (key : USize) (ls : list_t T) : Result T :=
+  (T : Type) (key : Usize) (ls : list_t T) : Result T :=
   do
     let t ⟵ hash_map_get_in_list_loop_fwd T key ls
     Result.ret t
 
 /- [hashmap::HashMap::{0}::get] -/
 def hash_map_get_fwd
-  (T : Type) (self : hash_map_t T) (key : USize) : Result T :=
+  (T : Type) (self : hash_map_t T) (key : Usize) : Result T :=
   do
     let hash ⟵ hash_key_fwd key
     let i := vec_len (list_t T) self.hash_map_slots
-    let hash_mod ⟵ USize.checked_rem hash i
+    let hash_mod ⟵ hash % i
     let l ⟵ vec_index_fwd (list_t T) self.hash_map_slots hash_mod
     hash_map_get_in_list_fwd T key l
 
 /- [hashmap::HashMap::{0}::get_mut_in_list] -/
 def hash_map_get_mut_in_list_loop_fwd
-  (T : Type) (ls : list_t T) (key : USize) : (Result T) :=
+  (T : Type) (ls : list_t T) (key : Usize) : (Result T) :=
   match 𝒽: ls with
-  | list_t.ListCons ckey cvalue tl =>
+  | list_t.Cons ckey cvalue tl =>
     if 𝒽: ckey = key
     then Result.ret cvalue
     else do
            let t ⟵ hash_map_get_mut_in_list_loop_fwd T tl key
            Result.ret t
-  | list_t.ListNil => Result.fail Error.panic
+  | list_t.Nil => Result.fail Error.panic
 termination_by hash_map_get_mut_in_list_loop_fwd ls key =>
   hash_map_get_mut_in_list_loop_terminates T ls key
 decreasing_by hash_map_get_mut_in_list_loop_decreases ls key
 
 /- [hashmap::HashMap::{0}::get_mut_in_list] -/
 def hash_map_get_mut_in_list_fwd
-  (T : Type) (ls : list_t T) (key : USize) : Result T :=
+  (T : Type) (ls : list_t T) (key : Usize) : Result T :=
   do
     let t ⟵ hash_map_get_mut_in_list_loop_fwd T ls key
     Result.ret t
 
 /- [hashmap::HashMap::{0}::get_mut_in_list] -/
 def hash_map_get_mut_in_list_loop_back
-  (T : Type) (ls : list_t T) (key : USize) (ret0 : T) : (Result (list_t T)) :=
+  (T : Type) (ls : list_t T) (key : Usize) (ret0 : T) : (Result (list_t T)) :=
   match 𝒽: ls with
-  | list_t.ListCons ckey cvalue tl =>
+  | list_t.Cons ckey cvalue tl =>
     if 𝒽: ckey = key
-    then Result.ret (list_t.ListCons ckey ret0 tl)
+    then Result.ret (list_t.Cons ckey ret0 tl)
     else
       do
         let tl0 ⟵ hash_map_get_mut_in_list_loop_back T tl key ret0
-        Result.ret (list_t.ListCons ckey cvalue tl0)
-  | list_t.ListNil => Result.fail Error.panic
+        Result.ret (list_t.Cons ckey cvalue tl0)
+  | list_t.Nil => Result.fail Error.panic
 termination_by hash_map_get_mut_in_list_loop_back ls key ret0 =>
   hash_map_get_mut_in_list_loop_terminates T ls key
 decreasing_by hash_map_get_mut_in_list_loop_decreases ls key
 
 /- [hashmap::HashMap::{0}::get_mut_in_list] -/
 def hash_map_get_mut_in_list_back
-  (T : Type) (ls : list_t T) (key : USize) (ret0 : T) : Result (list_t T) :=
+  (T : Type) (ls : list_t T) (key : Usize) (ret0 : T) : Result (list_t T) :=
   do
     let l ⟵ hash_map_get_mut_in_list_loop_back T ls key ret0
     Result.ret l
 
 /- [hashmap::HashMap::{0}::get_mut] -/
 def hash_map_get_mut_fwd
-  (T : Type) (self : hash_map_t T) (key : USize) : Result T :=
+  (T : Type) (self : hash_map_t T) (key : Usize) : Result T :=
   do
     let hash ⟵ hash_key_fwd key
     let i := vec_len (list_t T) self.hash_map_slots
-    let hash_mod ⟵ USize.checked_rem hash i
+    let hash_mod ⟵ hash % i
     let l ⟵ vec_index_mut_fwd (list_t T) self.hash_map_slots hash_mod
     hash_map_get_mut_in_list_fwd T l key
 
 /- [hashmap::HashMap::{0}::get_mut] -/
 def hash_map_get_mut_back
-  (T : Type) (self : hash_map_t T) (key : USize) (ret0 : T) :
+  (T : Type) (self : hash_map_t T) (key : Usize) (ret0 : T) :
   Result (hash_map_t T)
   :=
   do
     let hash ⟵ hash_key_fwd key
     let i := vec_len (list_t T) self.hash_map_slots
-    let hash_mod ⟵ USize.checked_rem hash i
+    let hash_mod ⟵ hash % i
     let l ⟵ vec_index_mut_fwd (list_t T) self.hash_map_slots hash_mod
     let l0 ⟵ hash_map_get_mut_in_list_back T l key ret0
     let v ⟵ vec_index_mut_back (list_t T) self.hash_map_slots hash_mod l0
-    Result.ret
-      {
-        hash_map_num_entries := self.hash_map_num_entries,
-        hash_map_max_load_factor := self.hash_map_max_load_factor,
-        hash_map_max_load := self.hash_map_max_load,
-        hash_map_slots := v
-      }
+    Result.ret { self with hash_map_slots := v }
 
 /- [hashmap::HashMap::{0}::remove_from_list] -/
 def hash_map_remove_from_list_loop_fwd
-  (T : Type) (key : USize) (ls : list_t T) : (Result (Option T)) :=
+  (T : Type) (key : Usize) (ls : list_t T) : (Result (Option T)) :=
   match 𝒽: ls with
-  | list_t.ListCons ckey t tl =>
+  | list_t.Cons ckey t tl =>
     if 𝒽: ckey = key
     then
       let mv_ls :=
-        mem_replace_fwd (list_t T) (list_t.ListCons ckey t tl) list_t.ListNil
+        mem_replace_fwd (list_t T) (list_t.Cons ckey t tl) list_t.Nil
       match 𝒽: mv_ls with
-      | list_t.ListCons i cvalue tl0 => Result.ret (Option.some cvalue)
-      | list_t.ListNil => Result.fail Error.panic
+      | list_t.Cons i cvalue tl0 => Result.ret (Option.some cvalue)
+      | list_t.Nil => Result.fail Error.panic
     else
       do
         let opt ⟵ hash_map_remove_from_list_loop_fwd T key tl
         Result.ret opt
-  | list_t.ListNil => Result.ret Option.none
+  | list_t.Nil => Result.ret Option.none
 termination_by hash_map_remove_from_list_loop_fwd key ls =>
   hash_map_remove_from_list_loop_terminates T key ls
 decreasing_by hash_map_remove_from_list_loop_decreases key ls
 
 /- [hashmap::HashMap::{0}::remove_from_list] -/
 def hash_map_remove_from_list_fwd
-  (T : Type) (key : USize) (ls : list_t T) : Result (Option T) :=
+  (T : Type) (key : Usize) (ls : list_t T) : Result (Option T) :=
   do
     let opt ⟵ hash_map_remove_from_list_loop_fwd T key ls
     Result.ret opt
 
 /- [hashmap::HashMap::{0}::remove_from_list] -/
 def hash_map_remove_from_list_loop_back
-  (T : Type) (key : USize) (ls : list_t T) : (Result (list_t T)) :=
+  (T : Type) (key : Usize) (ls : list_t T) : (Result (list_t T)) :=
   match 𝒽: ls with
-  | list_t.ListCons ckey t tl =>
+  | list_t.Cons ckey t tl =>
     if 𝒽: ckey = key
     then
       let mv_ls :=
-        mem_replace_fwd (list_t T) (list_t.ListCons ckey t tl) list_t.ListNil
+        mem_replace_fwd (list_t T) (list_t.Cons ckey t tl) list_t.Nil
       match 𝒽: mv_ls with
-      | list_t.ListCons i cvalue tl0 => Result.ret tl0
-      | list_t.ListNil => Result.fail Error.panic
+      | list_t.Cons i cvalue tl0 => Result.ret tl0
+      | list_t.Nil => Result.fail Error.panic
     else
       do
         let tl0 ⟵ hash_map_remove_from_list_loop_back T key tl
-        Result.ret (list_t.ListCons ckey t tl0)
-  | list_t.ListNil => Result.ret list_t.ListNil
+        Result.ret (list_t.Cons ckey t tl0)
+  | list_t.Nil => Result.ret list_t.Nil
 termination_by hash_map_remove_from_list_loop_back key ls =>
   hash_map_remove_from_list_loop_terminates T key ls
 decreasing_by hash_map_remove_from_list_loop_decreases key ls
 
 /- [hashmap::HashMap::{0}::remove_from_list] -/
 def hash_map_remove_from_list_back
-  (T : Type) (key : USize) (ls : list_t T) : Result (list_t T) :=
+  (T : Type) (key : Usize) (ls : list_t T) : Result (list_t T) :=
   do
     let l ⟵ hash_map_remove_from_list_loop_back T key ls
     Result.ret l
 
 /- [hashmap::HashMap::{0}::remove] -/
 def hash_map_remove_fwd
-  (T : Type) (self : hash_map_t T) (key : USize) : Result (Option T) :=
+  (T : Type) (self : hash_map_t T) (key : Usize) : Result (Option T) :=
   do
     let hash ⟵ hash_key_fwd key
     let i := vec_len (list_t T) self.hash_map_slots
-    let hash_mod ⟵ USize.checked_rem hash i
+    let hash_mod ⟵ hash % i
     let l ⟵ vec_index_mut_fwd (list_t T) self.hash_map_slots hash_mod
     let x ⟵ hash_map_remove_from_list_fwd T key l
     match 𝒽: x with
     | Option.none => Result.ret Option.none
     | Option.some x0 =>
       do
-        let _ ⟵ USize.checked_sub self.hash_map_num_entries
-          (USize.ofNatCore 1 (by intlit))
+        let _ ⟵ self.hash_map_num_entries - (Usize.ofInt 1 (by intlit))
         Result.ret (Option.some x0)
 
 /- [hashmap::HashMap::{0}::remove] -/
 def hash_map_remove_back
-  (T : Type) (self : hash_map_t T) (key : USize) : Result (hash_map_t T) :=
+  (T : Type) (self : hash_map_t T) (key : Usize) : Result (hash_map_t T) :=
   do
     let hash ⟵ hash_key_fwd key
     let i := vec_len (list_t T) self.hash_map_slots
-    let hash_mod ⟵ USize.checked_rem hash i
+    let hash_mod ⟵ hash % i
     let l ⟵ vec_index_mut_fwd (list_t T) self.hash_map_slots hash_mod
     let x ⟵ hash_map_remove_from_list_fwd T key l
     match 𝒽: x with
@@ -511,90 +490,71 @@ def hash_map_remove_back
       do
         let l0 ⟵ hash_map_remove_from_list_back T key l
         let v ⟵ vec_index_mut_back (list_t T) self.hash_map_slots hash_mod l0
-        Result.ret
-          {
-            hash_map_num_entries := self.hash_map_num_entries,
-            hash_map_max_load_factor := self.hash_map_max_load_factor,
-            hash_map_max_load := self.hash_map_max_load,
-            hash_map_slots := v
-          }
+        Result.ret { self with hash_map_slots := v }
     | Option.some x0 =>
       do
-        let i0 ⟵ USize.checked_sub self.hash_map_num_entries
-          (USize.ofNatCore 1 (by intlit))
+        let i0 ⟵ self.hash_map_num_entries - (Usize.ofInt 1 (by intlit))
         let l0 ⟵ hash_map_remove_from_list_back T key l
         let v ⟵ vec_index_mut_back (list_t T) self.hash_map_slots hash_mod l0
         Result.ret
-          {
-            hash_map_num_entries := i0,
-            hash_map_max_load_factor := self.hash_map_max_load_factor,
-            hash_map_max_load := self.hash_map_max_load,
-            hash_map_slots := v
-          }
+          { self with hash_map_num_entries := i0, hash_map_slots := v }
 
 /- [hashmap::test1] -/
 def test1_fwd : Result Unit :=
   do
-    let hm ⟵ hash_map_new_fwd UInt64
+    let hm ⟵ hash_map_new_fwd U64
     let hm0 ⟵
-      hash_map_insert_fwd_back UInt64 hm (USize.ofNatCore 0 (by intlit))
-        (UInt64.ofNatCore 42 (by intlit))
+      hash_map_insert_fwd_back U64 hm (Usize.ofInt 0 (by intlit))
+        (U64.ofInt 42 (by intlit))
     let hm1 ⟵
-      hash_map_insert_fwd_back UInt64 hm0 (USize.ofNatCore 128 (by intlit))
-        (UInt64.ofNatCore 18 (by intlit))
+      hash_map_insert_fwd_back U64 hm0 (Usize.ofInt 128 (by intlit))
+        (U64.ofInt 18 (by intlit))
     let hm2 ⟵
-      hash_map_insert_fwd_back UInt64 hm1 (USize.ofNatCore 1024 (by intlit))
-        (UInt64.ofNatCore 138 (by intlit))
+      hash_map_insert_fwd_back U64 hm1 (Usize.ofInt 1024 (by intlit))
+        (U64.ofInt 138 (by intlit))
     let hm3 ⟵
-      hash_map_insert_fwd_back UInt64 hm2 (USize.ofNatCore 1056 (by intlit))
-        (UInt64.ofNatCore 256 (by intlit))
-    let i ⟵ hash_map_get_fwd UInt64 hm3 (USize.ofNatCore 128 (by intlit))
-    if 𝒽: not (i = (UInt64.ofNatCore 18 (by intlit)))
+      hash_map_insert_fwd_back U64 hm2 (Usize.ofInt 1056 (by intlit))
+        (U64.ofInt 256 (by intlit))
+    let i ⟵ hash_map_get_fwd U64 hm3 (Usize.ofInt 128 (by intlit))
+    if 𝒽: not (i = (U64.ofInt 18 (by intlit)))
     then Result.fail Error.panic
     else
       do
         let hm4 ⟵
-          hash_map_get_mut_back UInt64 hm3 (USize.ofNatCore 1024 (by intlit))
-            (UInt64.ofNatCore 56 (by intlit))
-        let i0 ⟵
-          hash_map_get_fwd UInt64 hm4 (USize.ofNatCore 1024 (by intlit))
-        if 𝒽: not (i0 = (UInt64.ofNatCore 56 (by intlit)))
+          hash_map_get_mut_back U64 hm3 (Usize.ofInt 1024 (by intlit))
+            (U64.ofInt 56 (by intlit))
+        let i0 ⟵ hash_map_get_fwd U64 hm4 (Usize.ofInt 1024 (by intlit))
+        if 𝒽: not (i0 = (U64.ofInt 56 (by intlit)))
         then Result.fail Error.panic
         else
           do
             let x ⟵
-              hash_map_remove_fwd UInt64 hm4 (USize.ofNatCore 1024 (by intlit))
+              hash_map_remove_fwd U64 hm4 (Usize.ofInt 1024 (by intlit))
             match 𝒽: x with
             | Option.none => Result.fail Error.panic
             | Option.some x0 =>
-              if 𝒽: not (x0 = (UInt64.ofNatCore 56 (by intlit)))
+              if 𝒽: not (x0 = (U64.ofInt 56 (by intlit)))
               then Result.fail Error.panic
               else
                 do
                   let hm5 ⟵
-                    hash_map_remove_back UInt64 hm4
-                      (USize.ofNatCore 1024 (by intlit))
+                    hash_map_remove_back U64 hm4 (Usize.ofInt 1024 (by intlit))
                   let i1 ⟵
-                    hash_map_get_fwd UInt64 hm5 (USize.ofNatCore 0 (by intlit))
-                  if 𝒽: not (i1 = (UInt64.ofNatCore 42 (by intlit)))
+                    hash_map_get_fwd U64 hm5 (Usize.ofInt 0 (by intlit))
+                  if 𝒽: not (i1 = (U64.ofInt 42 (by intlit)))
                   then Result.fail Error.panic
                   else
                     do
                       let i2 ⟵
-                        hash_map_get_fwd UInt64 hm5
-                          (USize.ofNatCore 128 (by intlit))
-                      if 𝒽: not (i2 = (UInt64.ofNatCore 18 (by intlit)))
+                        hash_map_get_fwd U64 hm5 (Usize.ofInt 128 (by intlit))
+                      if 𝒽: not (i2 = (U64.ofInt 18 (by intlit)))
                       then Result.fail Error.panic
                       else
                         do
                           let i3 ⟵
-                            hash_map_get_fwd UInt64 hm5
-                              (USize.ofNatCore 1056 (by intlit))
-                          if 𝒽: not (i3 =
-                            (UInt64.ofNatCore 256 (by intlit)))
+                            hash_map_get_fwd U64 hm5
+                              (Usize.ofInt 1056 (by intlit))
+                          if 𝒽: not (i3 = (U64.ofInt 256 (by intlit)))
                           then Result.fail Error.panic
                           else Result.ret ()
-
-/- Unit test for [hashmap::test1] -/
-#assert (test1_fwd == .ret ())
 
