tests/lean/hashmap/Hashmap/Types.lean
@@ -4,15 +4,13 @@ import Base.Primitives
 
 /- [hashmap::List] -/
 inductive list_t (T : Type) :=
-| ListCons : USize -> T -> list_t T -> list_t T
-| ListNil : list_t T
+| Cons : Usize -> T -> list_t T -> list_t T
+| Nil : list_t T
 
 /- [hashmap::HashMap] -/
 structure hash_map_t (T : Type) where
-
-  hash_map_num_entries : USize
-  hash_map_max_load_factor : (USize × USize)
-  hash_map_max_load : USize
+  hash_map_num_entries : Usize
+  hash_map_max_load_factor : (Usize × Usize)
+  hash_map_max_load : Usize
   hash_map_slots : Vec (list_t T)
-
 
