tests/lean/hashmap_on_disk/HashmapMain/Clauses/Template.lean
@@ -6,34 +6,35 @@ import HashmapMain.Types
 /- [hashmap_main::hashmap::HashMap::{0}::allocate_slots]: termination measure -/
 @[simp]
 def hashmap_hash_map_allocate_slots_loop_terminates (T : Type)
-  (slots : Vec (hashmap_list_t T)) (n : USize) :=
+  (slots : Vec (hashmap_list_t T)) (n : Usize) :=
   (slots, n)
 
+/- [hashmap_main::hashmap::HashMap::{0}::allocate_slots]: decreases_by tactic -/
 syntax "hashmap_hash_map_allocate_slots_loop_decreases" term+ : tactic
-
 macro_rules
 | `(tactic| hashmap_hash_map_allocate_slots_loop_decreases $slots $n) =>
   `(tactic| sorry)
 
-/- [hashmap_main::hashmap::HashMap::{0}::clear]: termination measure -/
+/- [hashmap_main::hashmap::HashMap::{0}::clear_slots]: termination measure -/
 @[simp]
-def hashmap_hash_map_clear_loop_terminates (T : Type)
-  (slots : Vec (hashmap_list_t T)) (i : USize) :=
+def hashmap_hash_map_clear_slots_loop_terminates (T : Type)
+  (slots : Vec (hashmap_list_t T)) (i : Usize) :=
   (slots, i)
 
-syntax "hashmap_hash_map_clear_loop_decreases" term+ : tactic
-
+/- [hashmap_main::hashmap::HashMap::{0}::clear_slots]: decreases_by tactic -/
+syntax "hashmap_hash_map_clear_slots_loop_decreases" term+ : tactic
 macro_rules
-| `(tactic| hashmap_hash_map_clear_loop_decreases $slots $i) =>`(tactic| sorry)
+| `(tactic| hashmap_hash_map_clear_slots_loop_decreases $slots $i) =>
+  `(tactic| sorry)
 
 /- [hashmap_main::hashmap::HashMap::{0}::insert_in_list]: termination measure -/
 @[simp]
-def hashmap_hash_map_insert_in_list_loop_terminates (T : Type) (key : USize)
+def hashmap_hash_map_insert_in_list_loop_terminates (T : Type) (key : Usize)
   (value : T) (ls : hashmap_list_t T) :=
   (key, value, ls)
 
+/- [hashmap_main::hashmap::HashMap::{0}::insert_in_list]: decreases_by tactic -/
 syntax "hashmap_hash_map_insert_in_list_loop_decreases" term+ : tactic
-
 macro_rules
 | `(tactic| hashmap_hash_map_insert_in_list_loop_decreases $key $value $ls) =>
   `(tactic| sorry)
@@ -44,8 +45,8 @@ def hashmap_hash_map_move_elements_from_list_loop_terminates (T : Type)
   (ntable : hashmap_hash_map_t T) (ls : hashmap_list_t T) :=
   (ntable, ls)
 
+/- [hashmap_main::hashmap::HashMap::{0}::move_elements_from_list]: decreases_by tactic -/
 syntax "hashmap_hash_map_move_elements_from_list_loop_decreases" term+ : tactic
-
 macro_rules
 | `(tactic| hashmap_hash_map_move_elements_from_list_loop_decreases $ntable
 $ls) =>`(tactic| sorry)
@@ -53,12 +54,12 @@ $ls) =>`(tactic| sorry)
 /- [hashmap_main::hashmap::HashMap::{0}::move_elements]: termination measure -/
 @[simp]
 def hashmap_hash_map_move_elements_loop_terminates (T : Type)
-  (ntable : hashmap_hash_map_t T) (slots : Vec (hashmap_list_t T)) (i : USize)
+  (ntable : hashmap_hash_map_t T) (slots : Vec (hashmap_list_t T)) (i : Usize)
   :=
   (ntable, slots, i)
 
+/- [hashmap_main::hashmap::HashMap::{0}::move_elements]: decreases_by tactic -/
 syntax "hashmap_hash_map_move_elements_loop_decreases" term+ : tactic
-
 macro_rules
 | `(tactic| hashmap_hash_map_move_elements_loop_decreases $ntable $slots $i) =>
   `(tactic| sorry)
@@ -66,46 +67,46 @@ macro_rules
 /- [hashmap_main::hashmap::HashMap::{0}::contains_key_in_list]: termination measure -/
 @[simp]
 def hashmap_hash_map_contains_key_in_list_loop_terminates (T : Type)
-  (key : USize) (ls : hashmap_list_t T) :=
+  (key : Usize) (ls : hashmap_list_t T) :=
   (key, ls)
 
+/- [hashmap_main::hashmap::HashMap::{0}::contains_key_in_list]: decreases_by tactic -/
 syntax "hashmap_hash_map_contains_key_in_list_loop_decreases" term+ : tactic
-
 macro_rules
 | `(tactic| hashmap_hash_map_contains_key_in_list_loop_decreases $key $ls) =>
   `(tactic| sorry)
 
 /- [hashmap_main::hashmap::HashMap::{0}::get_in_list]: termination measure -/
 @[simp]
-def hashmap_hash_map_get_in_list_loop_terminates (T : Type) (key : USize)
+def hashmap_hash_map_get_in_list_loop_terminates (T : Type) (key : Usize)
   (ls : hashmap_list_t T) :=
   (key, ls)
 
+/- [hashmap_main::hashmap::HashMap::{0}::get_in_list]: decreases_by tactic -/
 syntax "hashmap_hash_map_get_in_list_loop_decreases" term+ : tactic
-
 macro_rules
 | `(tactic| hashmap_hash_map_get_in_list_loop_decreases $key $ls) =>`(tactic| sorry)
 
 /- [hashmap_main::hashmap::HashMap::{0}::get_mut_in_list]: termination measure -/
 @[simp]
 def hashmap_hash_map_get_mut_in_list_loop_terminates (T : Type)
-  (ls : hashmap_list_t T) (key : USize) :=
+  (ls : hashmap_list_t T) (key : Usize) :=
   (ls, key)
 
+/- [hashmap_main::hashmap::HashMap::{0}::get_mut_in_list]: decreases_by tactic -/
 syntax "hashmap_hash_map_get_mut_in_list_loop_decreases" term+ : tactic
-
 macro_rules
 | `(tactic| hashmap_hash_map_get_mut_in_list_loop_decreases $ls $key) =>
   `(tactic| sorry)
 
 /- [hashmap_main::hashmap::HashMap::{0}::remove_from_list]: termination measure -/
 @[simp]
-def hashmap_hash_map_remove_from_list_loop_terminates (T : Type) (key : USize)
+def hashmap_hash_map_remove_from_list_loop_terminates (T : Type) (key : Usize)
   (ls : hashmap_list_t T) :=
   (key, ls)
 
+/- [hashmap_main::hashmap::HashMap::{0}::remove_from_list]: decreases_by tactic -/
 syntax "hashmap_hash_map_remove_from_list_loop_decreases" term+ : tactic
-
 macro_rules
 | `(tactic| hashmap_hash_map_remove_from_list_loop_decreases $key $ls) =>
   `(tactic| sorry)
