tests/lean/misc-loops/Loops/Funs.lean
@@ -6,29 +6,34 @@ import Loops.Clauses.Clauses
 
 /- [loops::sum] -/
 def sum_loop_fwd (max : U32) (i : U32) (s : U32) : (Result U32) :=
-  if h: i < max
+  if 𝒽: i < max
   then
     do
-      let s0 ← s + i
-      let i0 ← i + (U32.ofInt 1 (by intlit))
-      sum_loop_fwd max i0 s0
+      let s0 ⟵ s + i
+      let i0 ⟵ i + (U32.ofInt 1 (by intlit))
+      let i1 ⟵ sum_loop_fwd max i0 s0
+      Result.ret i1
   else s * (U32.ofInt 2 (by intlit))
 termination_by sum_loop_fwd max i s => sum_loop_terminates max i s
 decreasing_by sum_loop_decreases max i s
 
 /- [loops::sum] -/
 def sum_fwd (max : U32) : Result U32 :=
-  sum_loop_fwd max (U32.ofInt 0 (by intlit)) (U32.ofInt 0 (by intlit))
+  do
+    let i ⟵
+      sum_loop_fwd max (U32.ofInt 0 (by intlit)) (U32.ofInt 0 (by intlit))
+    Result.ret i
 
 /- [loops::sum_with_mut_borrows] -/
 def sum_with_mut_borrows_loop_fwd
   (max : U32) (mi : U32) (ms : U32) : (Result U32) :=
-  if h: mi < max
+  if 𝒽: mi < max
   then
     do
-      let ms0 ← ms + mi
-      let mi0 ← mi + (U32.ofInt 1 (by intlit))
-      sum_with_mut_borrows_loop_fwd max mi0 ms0
+      let ms0 ⟵ ms + mi
+      let mi0 ⟵ mi + (U32.ofInt 1 (by intlit))
+      let i ⟵ sum_with_mut_borrows_loop_fwd max mi0 ms0
+      Result.ret i
   else ms * (U32.ofInt 2 (by intlit))
 termination_by sum_with_mut_borrows_loop_fwd max mi ms =>
   sum_with_mut_borrows_loop_terminates max mi ms
@@ -36,18 +41,22 @@ decreasing_by sum_with_mut_borrows_loop_decreases max mi ms
 
 /- [loops::sum_with_mut_borrows] -/
 def sum_with_mut_borrows_fwd (max : U32) : Result U32 :=
-  sum_with_mut_borrows_loop_fwd max (U32.ofInt 0 (by intlit))
-    (U32.ofInt 0 (by intlit))
+  do
+    let i ⟵
+      sum_with_mut_borrows_loop_fwd max (U32.ofInt 0 (by intlit))
+        (U32.ofInt 0 (by intlit))
+    Result.ret i
 
 /- [loops::sum_with_shared_borrows] -/
 def sum_with_shared_borrows_loop_fwd
   (max : U32) (i : U32) (s : U32) : (Result U32) :=
-  if h: i < max
+  if 𝒽: i < max
   then
     do
-      let i0 ← i + (U32.ofInt 1 (by intlit))
-      let s0 ← s + i0
-      sum_with_shared_borrows_loop_fwd max i0 s0
+      let i0 ⟵ i + (U32.ofInt 1 (by intlit))
+      let s0 ⟵ s + i0
+      let i1 ⟵ sum_with_shared_borrows_loop_fwd max i0 s0
+      Result.ret i1
   else s * (U32.ofInt 2 (by intlit))
 termination_by sum_with_shared_borrows_loop_fwd max i s =>
   sum_with_shared_borrows_loop_terminates max i s
@@ -55,52 +64,63 @@ decreasing_by sum_with_shared_borrows_loop_decreases max i s
 
 /- [loops::sum_with_shared_borrows] -/
 def sum_with_shared_borrows_fwd (max : U32) : Result U32 :=
-  sum_with_shared_borrows_loop_fwd max (U32.ofInt 0 (by intlit))
-    (U32.ofInt 0 (by intlit))
+  do
+    let i ⟵
+      sum_with_shared_borrows_loop_fwd max (U32.ofInt 0 (by intlit))
+        (U32.ofInt 0 (by intlit))
+    Result.ret i
 
 /- [loops::clear] -/
 def clear_loop_fwd_back (v : Vec U32) (i : Usize) : (Result (Vec U32)) :=
   let i0 := vec_len U32 v
-  if h: i < i0
+  if 𝒽: i < i0
   then
     do
-      let i1 ← i + (Usize.ofInt 1 (by intlit))
-      let v0 ← vec_index_mut_back U32 v i (U32.ofInt 0 (by intlit))
-      clear_loop_fwd_back v0 i1
+      let i1 ⟵ i + (Usize.ofInt 1 (by intlit))
+      let v0 ⟵ vec_index_mut_back U32 v i (U32.ofInt 0 (by intlit))
+      let v1 ⟵ clear_loop_fwd_back v0 i1
+      Result.ret v1
   else Result.ret v
 termination_by clear_loop_fwd_back v i => clear_loop_terminates v i
 decreasing_by clear_loop_decreases v i
 
 /- [loops::clear] -/
 def clear_fwd_back (v : Vec U32) : Result (Vec U32) :=
-  clear_loop_fwd_back v (Usize.ofInt 0 (by intlit))
+  do
+    let v0 ⟵ clear_loop_fwd_back v (Usize.ofInt 0 (by intlit))
+    Result.ret v0
 
 /- [loops::list_mem] -/
 def list_mem_loop_fwd (x : U32) (ls : list_t U32) : (Result Bool) :=
-  match h: ls with
+  match 𝒽: ls with
   | list_t.Cons y tl =>
-    if h: y = x
+    if 𝒽: y = x
     then Result.ret true
-    else list_mem_loop_fwd x tl
+    else do
+           let b ⟵ list_mem_loop_fwd x tl
+           Result.ret b
   | list_t.Nil => Result.ret false
 termination_by list_mem_loop_fwd x ls => list_mem_loop_terminates x ls
 decreasing_by list_mem_loop_decreases x ls
 
 /- [loops::list_mem] -/
 def list_mem_fwd (x : U32) (ls : list_t U32) : Result Bool :=
-  list_mem_loop_fwd x ls
+  do
+    let b ⟵ list_mem_loop_fwd x ls
+    Result.ret b
 
 /- [loops::list_nth_mut_loop] -/
 def list_nth_mut_loop_loop_fwd
   (T : Type) (ls : list_t T) (i : U32) : (Result T) :=
-  match h: ls with
+  match 𝒽: ls with
   | list_t.Cons x tl =>
-    if h: i = (U32.ofInt 0 (by intlit))
+    if 𝒽: i = (U32.ofInt 0 (by intlit))
     then Result.ret x
     else
       do
-        let i0 ← i - (U32.ofInt 1 (by intlit))
-        list_nth_mut_loop_loop_fwd T tl i0
+        let i0 ⟵ i - (U32.ofInt 1 (by intlit))
+        let t ⟵ list_nth_mut_loop_loop_fwd T tl i0
+        Result.ret t
   | list_t.Nil => Result.fail Error.panic
 termination_by list_nth_mut_loop_loop_fwd ls i =>
   list_nth_mut_loop_loop_terminates T ls i
@@ -108,19 +128,21 @@ decreasing_by list_nth_mut_loop_loop_decreases ls i
 
 /- [loops::list_nth_mut_loop] -/
 def list_nth_mut_loop_fwd (T : Type) (ls : list_t T) (i : U32) : Result T :=
-  list_nth_mut_loop_loop_fwd T ls i
+  do
+    let t ⟵ list_nth_mut_loop_loop_fwd T ls i
+    Result.ret t
 
 /- [loops::list_nth_mut_loop] -/
 def list_nth_mut_loop_loop_back
   (T : Type) (ls : list_t T) (i : U32) (ret0 : T) : (Result (list_t T)) :=
-  match h: ls with
+  match 𝒽: ls with
   | list_t.Cons x tl =>
-    if h: i = (U32.ofInt 0 (by intlit))
+    if 𝒽: i = (U32.ofInt 0 (by intlit))
     then Result.ret (list_t.Cons ret0 tl)
     else
       do
-        let i0 ← i - (U32.ofInt 1 (by intlit))
-        let tl0 ← list_nth_mut_loop_loop_back T tl i0 ret0
+        let i0 ⟵ i - (U32.ofInt 1 (by intlit))
+        let tl0 ⟵ list_nth_mut_loop_loop_back T tl i0 ret0
         Result.ret (list_t.Cons x tl0)
   | list_t.Nil => Result.fail Error.panic
 termination_by list_nth_mut_loop_loop_back ls i ret0 =>
@@ -130,19 +152,22 @@ decreasing_by list_nth_mut_loop_loop_decreases ls i
 /- [loops::list_nth_mut_loop] -/
 def list_nth_mut_loop_back
   (T : Type) (ls : list_t T) (i : U32) (ret0 : T) : Result (list_t T) :=
-  list_nth_mut_loop_loop_back T ls i ret0
+  do
+    let l ⟵ list_nth_mut_loop_loop_back T ls i ret0
+    Result.ret l
 
 /- [loops::list_nth_shared_loop] -/
 def list_nth_shared_loop_loop_fwd
   (T : Type) (ls : list_t T) (i : U32) : (Result T) :=
-  match h: ls with
+  match 𝒽: ls with
   | list_t.Cons x tl =>
-    if h: i = (U32.ofInt 0 (by intlit))
+    if 𝒽: i = (U32.ofInt 0 (by intlit))
     then Result.ret x
     else
       do
-        let i0 ← i - (U32.ofInt 1 (by intlit))
-        list_nth_shared_loop_loop_fwd T tl i0
+        let i0 ⟵ i - (U32.ofInt 1 (by intlit))
+        let t ⟵ list_nth_shared_loop_loop_fwd T tl i0
+        Result.ret t
   | list_t.Nil => Result.fail Error.panic
 termination_by list_nth_shared_loop_loop_fwd ls i =>
   list_nth_shared_loop_loop_terminates T ls i
@@ -150,15 +175,19 @@ decreasing_by list_nth_shared_loop_loop_decreases ls i
 
 /- [loops::list_nth_shared_loop] -/
 def list_nth_shared_loop_fwd (T : Type) (ls : list_t T) (i : U32) : Result T :=
-  list_nth_shared_loop_loop_fwd T ls i
+  do
+    let t ⟵ list_nth_shared_loop_loop_fwd T ls i
+    Result.ret t
 
 /- [loops::get_elem_mut] -/
 def get_elem_mut_loop_fwd (x : Usize) (ls : list_t Usize) : (Result Usize) :=
-  match h: ls with
+  match 𝒽: ls with
   | list_t.Cons y tl =>
-    if h: y = x
+    if 𝒽: y = x
     then Result.ret y
-    else get_elem_mut_loop_fwd x tl
+    else do
+           let i ⟵ get_elem_mut_loop_fwd x tl
+           Result.ret i
   | list_t.Nil => Result.fail Error.panic
 termination_by get_elem_mut_loop_fwd x ls => get_elem_mut_loop_terminates x ls
 decreasing_by get_elem_mut_loop_decreases x ls
@@ -166,20 +195,21 @@ decreasing_by get_elem_mut_loop_decreases x ls
 /- [loops::get_elem_mut] -/
 def get_elem_mut_fwd (slots : Vec (list_t Usize)) (x : Usize) : Result Usize :=
   do
-    let l ←
+    let l ⟵
       vec_index_mut_fwd (list_t Usize) slots (Usize.ofInt 0 (by intlit))
-    get_elem_mut_loop_fwd x l
+    let i ⟵ get_elem_mut_loop_fwd x l
+    Result.ret i
 
 /- [loops::get_elem_mut] -/
 def get_elem_mut_loop_back
   (x : Usize) (ls : list_t Usize) (ret0 : Usize) : (Result (list_t Usize)) :=
-  match h: ls with
+  match 𝒽: ls with
   | list_t.Cons y tl =>
-    if h: y = x
+    if 𝒽: y = x
     then Result.ret (list_t.Cons ret0 tl)
     else
       do
-        let tl0 ← get_elem_mut_loop_back x tl ret0
+        let tl0 ⟵ get_elem_mut_loop_back x tl ret0
         Result.ret (list_t.Cons y tl0)
   | list_t.Nil => Result.fail Error.panic
 termination_by get_elem_mut_loop_back x ls ret0 =>
@@ -192,19 +222,21 @@ def get_elem_mut_back
   Result (Vec (list_t Usize))
   :=
   do
-    let l ←
+    let l ⟵
       vec_index_mut_fwd (list_t Usize) slots (Usize.ofInt 0 (by intlit))
-    let l0 ← get_elem_mut_loop_back x l ret0
+    let l0 ⟵ get_elem_mut_loop_back x l ret0
     vec_index_mut_back (list_t Usize) slots (Usize.ofInt 0 (by intlit)) l0
 
 /- [loops::get_elem_shared] -/
 def get_elem_shared_loop_fwd
   (x : Usize) (ls : list_t Usize) : (Result Usize) :=
-  match h: ls with
+  match 𝒽: ls with
   | list_t.Cons y tl =>
-    if h: y = x
+    if 𝒽: y = x
     then Result.ret y
-    else get_elem_shared_loop_fwd x tl
+    else do
+           let i ⟵ get_elem_shared_loop_fwd x tl
+           Result.ret i
   | list_t.Nil => Result.fail Error.panic
 termination_by get_elem_shared_loop_fwd x ls =>
   get_elem_shared_loop_terminates x ls
@@ -214,8 +246,9 @@ decreasing_by get_elem_shared_loop_decreases x ls
 def get_elem_shared_fwd
   (slots : Vec (list_t Usize)) (x : Usize) : Result Usize :=
   do
-    let l ← vec_index_fwd (list_t Usize) slots (Usize.ofInt 0 (by intlit))
-    get_elem_shared_loop_fwd x l
+    let l ⟵ vec_index_fwd (list_t Usize) slots (Usize.ofInt 0 (by intlit))
+    let i ⟵ get_elem_shared_loop_fwd x l
+    Result.ret i
 
 /- [loops::id_mut] -/
 def id_mut_fwd (T : Type) (ls : list_t T) : Result (list_t T) :=
@@ -233,14 +266,15 @@ def id_shared_fwd (T : Type) (ls : list_t T) : Result (list_t T) :=
 /- [loops::list_nth_mut_loop_with_id] -/
 def list_nth_mut_loop_with_id_loop_fwd
   (T : Type) (i : U32) (ls : list_t T) : (Result T) :=
-  match h: ls with
+  match 𝒽: ls with
   | list_t.Cons x tl =>
-    if h: i = (U32.ofInt 0 (by intlit))
+    if 𝒽: i = (U32.ofInt 0 (by intlit))
     then Result.ret x
     else
       do
-        let i0 ← i - (U32.ofInt 1 (by intlit))
-        list_nth_mut_loop_with_id_loop_fwd T i0 tl
+        let i0 ⟵ i - (U32.ofInt 1 (by intlit))
+        let t ⟵ list_nth_mut_loop_with_id_loop_fwd T i0 tl
+        Result.ret t
   | list_t.Nil => Result.fail Error.panic
 termination_by list_nth_mut_loop_with_id_loop_fwd i ls =>
   list_nth_mut_loop_with_id_loop_terminates T i ls
@@ -250,20 +284,21 @@ decreasing_by list_nth_mut_loop_with_id_loop_decreases i ls
 def list_nth_mut_loop_with_id_fwd
   (T : Type) (ls : list_t T) (i : U32) : Result T :=
   do
-    let ls0 ← id_mut_fwd T ls
-    list_nth_mut_loop_with_id_loop_fwd T i ls0
+    let ls0 ⟵ id_mut_fwd T ls
+    let t ⟵ list_nth_mut_loop_with_id_loop_fwd T i ls0
+    Result.ret t
 
 /- [loops::list_nth_mut_loop_with_id] -/
 def list_nth_mut_loop_with_id_loop_back
   (T : Type) (i : U32) (ls : list_t T) (ret0 : T) : (Result (list_t T)) :=
-  match h: ls with
+  match 𝒽: ls with
   | list_t.Cons x tl =>
-    if h: i = (U32.ofInt 0 (by intlit))
+    if 𝒽: i = (U32.ofInt 0 (by intlit))
     then Result.ret (list_t.Cons ret0 tl)
     else
       do
-        let i0 ← i - (U32.ofInt 1 (by intlit))
-        let tl0 ← list_nth_mut_loop_with_id_loop_back T i0 tl ret0
+        let i0 ⟵ i - (U32.ofInt 1 (by intlit))
+        let tl0 ⟵ list_nth_mut_loop_with_id_loop_back T i0 tl ret0
         Result.ret (list_t.Cons x tl0)
   | list_t.Nil => Result.fail Error.panic
 termination_by list_nth_mut_loop_with_id_loop_back i ls ret0 =>
@@ -274,21 +309,22 @@ decreasing_by list_nth_mut_loop_with_id_loop_decreases i ls
 def list_nth_mut_loop_with_id_back
   (T : Type) (ls : list_t T) (i : U32) (ret0 : T) : Result (list_t T) :=
   do
-    let ls0 ← id_mut_fwd T ls
-    let l ← list_nth_mut_loop_with_id_loop_back T i ls0 ret0
+    let ls0 ⟵ id_mut_fwd T ls
+    let l ⟵ list_nth_mut_loop_with_id_loop_back T i ls0 ret0
     id_mut_back T ls l
 
 /- [loops::list_nth_shared_loop_with_id] -/
 def list_nth_shared_loop_with_id_loop_fwd
   (T : Type) (i : U32) (ls : list_t T) : (Result T) :=
-  match h: ls with
+  match 𝒽: ls with
   | list_t.Cons x tl =>
-    if h: i = (U32.ofInt 0 (by intlit))
+    if 𝒽: i = (U32.ofInt 0 (by intlit))
     then Result.ret x
     else
       do
-        let i0 ← i - (U32.ofInt 1 (by intlit))
-        list_nth_shared_loop_with_id_loop_fwd T i0 tl
+        let i0 ⟵ i - (U32.ofInt 1 (by intlit))
+        let t ⟵ list_nth_shared_loop_with_id_loop_fwd T i0 tl
+        Result.ret t
   | list_t.Nil => Result.fail Error.panic
 termination_by list_nth_shared_loop_with_id_loop_fwd i ls =>
   list_nth_shared_loop_with_id_loop_terminates T i ls
@@ -298,22 +334,24 @@ decreasing_by list_nth_shared_loop_with_id_loop_decreases i ls
 def list_nth_shared_loop_with_id_fwd
   (T : Type) (ls : list_t T) (i : U32) : Result T :=
   do
-    let ls0 ← id_shared_fwd T ls
-    list_nth_shared_loop_with_id_loop_fwd T i ls0
+    let ls0 ⟵ id_shared_fwd T ls
+    let t ⟵ list_nth_shared_loop_with_id_loop_fwd T i ls0
+    Result.ret t
 
 /- [loops::list_nth_mut_loop_pair] -/
 def list_nth_mut_loop_pair_loop_fwd
   (T : Type) (ls0 : list_t T) (ls1 : list_t T) (i : U32) : (Result (T × T)) :=
-  match h: ls0 with
+  match 𝒽: ls0 with
   | list_t.Cons x0 tl0 =>
-    match h: ls1 with
+    match 𝒽: ls1 with
     | list_t.Cons x1 tl1 =>
-      if h: i = (U32.ofInt 0 (by intlit))
+      if 𝒽: i = (U32.ofInt 0 (by intlit))
       then Result.ret (x0, x1)
       else
         do
-          let i0 ← i - (U32.ofInt 1 (by intlit))
-          list_nth_mut_loop_pair_loop_fwd T tl0 tl1 i0
+          let i0 ⟵ i - (U32.ofInt 1 (by intlit))
+          let p ⟵ list_nth_mut_loop_pair_loop_fwd T tl0 tl1 i0
+          Result.ret p
     | list_t.Nil => Result.fail Error.panic
   | list_t.Nil => Result.fail Error.panic
 termination_by list_nth_mut_loop_pair_loop_fwd ls0 ls1 i =>
@@ -323,23 +361,25 @@ decreasing_by list_nth_mut_loop_pair_loop_decreases ls0 ls1 i
 /- [loops::list_nth_mut_loop_pair] -/
 def list_nth_mut_loop_pair_fwd
   (T : Type) (ls0 : list_t T) (ls1 : list_t T) (i : U32) : Result (T × T) :=
-  list_nth_mut_loop_pair_loop_fwd T ls0 ls1 i
+  do
+    let p ⟵ list_nth_mut_loop_pair_loop_fwd T ls0 ls1 i
+    Result.ret p
 
 /- [loops::list_nth_mut_loop_pair] -/
 def list_nth_mut_loop_pair_loop_back'a
   (T : Type) (ls0 : list_t T) (ls1 : list_t T) (i : U32) (ret0 : T) :
   (Result (list_t T))
   :=
-  match h: ls0 with
+  match 𝒽: ls0 with
   | list_t.Cons x0 tl0 =>
-    match h: ls1 with
+    match 𝒽: ls1 with
     | list_t.Cons x1 tl1 =>
-      if h: i = (U32.ofInt 0 (by intlit))
+      if 𝒽: i = (U32.ofInt 0 (by intlit))
       then Result.ret (list_t.Cons ret0 tl0)
       else
         do
-          let i0 ← i - (U32.ofInt 1 (by intlit))
-          let tl00 ← list_nth_mut_loop_pair_loop_back'a T tl0 tl1 i0 ret0
+          let i0 ⟵ i - (U32.ofInt 1 (by intlit))
+          let tl00 ⟵ list_nth_mut_loop_pair_loop_back'a T tl0 tl1 i0 ret0
           Result.ret (list_t.Cons x0 tl00)
     | list_t.Nil => Result.fail Error.panic
   | list_t.Nil => Result.fail Error.panic
@@ -352,23 +392,25 @@ def list_nth_mut_loop_pair_back'a
   (T : Type) (ls0 : list_t T) (ls1 : list_t T) (i : U32) (ret0 : T) :
   Result (list_t T)
   :=
-  list_nth_mut_loop_pair_loop_back'a T ls0 ls1 i ret0
+  do
+    let l ⟵ list_nth_mut_loop_pair_loop_back'a T ls0 ls1 i ret0
+    Result.ret l
 
 /- [loops::list_nth_mut_loop_pair] -/
 def list_nth_mut_loop_pair_loop_back'b
   (T : Type) (ls0 : list_t T) (ls1 : list_t T) (i : U32) (ret0 : T) :
   (Result (list_t T))
   :=
-  match h: ls0 with
+  match 𝒽: ls0 with
   | list_t.Cons x0 tl0 =>
-    match h: ls1 with
+    match 𝒽: ls1 with
     | list_t.Cons x1 tl1 =>
-      if h: i = (U32.ofInt 0 (by intlit))
+      if 𝒽: i = (U32.ofInt 0 (by intlit))
       then Result.ret (list_t.Cons ret0 tl1)
       else
         do
-          let i0 ← i - (U32.ofInt 1 (by intlit))
-          let tl10 ← list_nth_mut_loop_pair_loop_back'b T tl0 tl1 i0 ret0
+          let i0 ⟵ i - (U32.ofInt 1 (by intlit))
+          let tl10 ⟵ list_nth_mut_loop_pair_loop_back'b T tl0 tl1 i0 ret0
           Result.ret (list_t.Cons x1 tl10)
     | list_t.Nil => Result.fail Error.panic
   | list_t.Nil => Result.fail Error.panic
@@ -381,21 +423,24 @@ def list_nth_mut_loop_pair_back'b
   (T : Type) (ls0 : list_t T) (ls1 : list_t T) (i : U32) (ret0 : T) :
   Result (list_t T)
   :=
-  list_nth_mut_loop_pair_loop_back'b T ls0 ls1 i ret0
+  do
+    let l ⟵ list_nth_mut_loop_pair_loop_back'b T ls0 ls1 i ret0
+    Result.ret l
 
 /- [loops::list_nth_shared_loop_pair] -/
 def list_nth_shared_loop_pair_loop_fwd
   (T : Type) (ls0 : list_t T) (ls1 : list_t T) (i : U32) : (Result (T × T)) :=
-  match h: ls0 with
+  match 𝒽: ls0 with
   | list_t.Cons x0 tl0 =>
-    match h: ls1 with
+    match 𝒽: ls1 with
     | list_t.Cons x1 tl1 =>
-      if h: i = (U32.ofInt 0 (by intlit))
+      if 𝒽: i = (U32.ofInt 0 (by intlit))
       then Result.ret (x0, x1)
       else
         do
-          let i0 ← i - (U32.ofInt 1 (by intlit))
-          list_nth_shared_loop_pair_loop_fwd T tl0 tl1 i0
+          let i0 ⟵ i - (U32.ofInt 1 (by intlit))
+          let p ⟵ list_nth_shared_loop_pair_loop_fwd T tl0 tl1 i0
+          Result.ret p
     | list_t.Nil => Result.fail Error.panic
   | list_t.Nil => Result.fail Error.panic
 termination_by list_nth_shared_loop_pair_loop_fwd ls0 ls1 i =>
@@ -405,21 +450,24 @@ decreasing_by list_nth_shared_loop_pair_loop_decreases ls0 ls1 i
 /- [loops::list_nth_shared_loop_pair] -/
 def list_nth_shared_loop_pair_fwd
   (T : Type) (ls0 : list_t T) (ls1 : list_t T) (i : U32) : Result (T × T) :=
-  list_nth_shared_loop_pair_loop_fwd T ls0 ls1 i
+  do
+    let p ⟵ list_nth_shared_loop_pair_loop_fwd T ls0 ls1 i
+    Result.ret p
 
 /- [loops::list_nth_mut_loop_pair_merge] -/
 def list_nth_mut_loop_pair_merge_loop_fwd
   (T : Type) (ls0 : list_t T) (ls1 : list_t T) (i : U32) : (Result (T × T)) :=
-  match h: ls0 with
+  match 𝒽: ls0 with
   | list_t.Cons x0 tl0 =>
-    match h: ls1 with
+    match 𝒽: ls1 with
     | list_t.Cons x1 tl1 =>
-      if h: i = (U32.ofInt 0 (by intlit))
+      if 𝒽: i = (U32.ofInt 0 (by intlit))
       then Result.ret (x0, x1)
       else
         do
-          let i0 ← i - (U32.ofInt 1 (by intlit))
-          list_nth_mut_loop_pair_merge_loop_fwd T tl0 tl1 i0
+          let i0 ⟵ i - (U32.ofInt 1 (by intlit))
+          let p ⟵ list_nth_mut_loop_pair_merge_loop_fwd T tl0 tl1 i0
+          Result.ret p
     | list_t.Nil => Result.fail Error.panic
   | list_t.Nil => Result.fail Error.panic
 termination_by list_nth_mut_loop_pair_merge_loop_fwd ls0 ls1 i =>
@@ -429,26 +477,28 @@ decreasing_by list_nth_mut_loop_pair_merge_loop_decreases ls0 ls1 i
 /- [loops::list_nth_mut_loop_pair_merge] -/
 def list_nth_mut_loop_pair_merge_fwd
   (T : Type) (ls0 : list_t T) (ls1 : list_t T) (i : U32) : Result (T × T) :=
-  list_nth_mut_loop_pair_merge_loop_fwd T ls0 ls1 i
+  do
+    let p ⟵ list_nth_mut_loop_pair_merge_loop_fwd T ls0 ls1 i
+    Result.ret p
 
 /- [loops::list_nth_mut_loop_pair_merge] -/
 def list_nth_mut_loop_pair_merge_loop_back
   (T : Type) (ls0 : list_t T) (ls1 : list_t T) (i : U32) (ret0 : (T × T)) :
   (Result ((list_t T) × (list_t T)))
   :=
-  match h: ls0 with
+  match 𝒽: ls0 with
   | list_t.Cons x0 tl0 =>
-    match h: ls1 with
+    match 𝒽: ls1 with
     | list_t.Cons x1 tl1 =>
-      if h: i = (U32.ofInt 0 (by intlit))
+      if 𝒽: i = (U32.ofInt 0 (by intlit))
       then
         let (t, t0) := ret0
         Result.ret (list_t.Cons t tl0, list_t.Cons t0 tl1)
       else
         do
-          let i0 ← i - (U32.ofInt 1 (by intlit))
-          let (tl00, tl10) ←
-            list_nth_mut_loop_pair_merge_loop_back T tl0 tl1 i0 ret0
+          let i0 ⟵ i - (U32.ofInt 1 (by intlit))
+          let p ⟵ list_nth_mut_loop_pair_merge_loop_back T tl0 tl1 i0 ret0
+          let (tl00, tl10) := p
           Result.ret (list_t.Cons x0 tl00, list_t.Cons x1 tl10)
     | list_t.Nil => Result.fail Error.panic
   | list_t.Nil => Result.fail Error.panic
@@ -461,21 +511,25 @@ def list_nth_mut_loop_pair_merge_back
   (T : Type) (ls0 : list_t T) (ls1 : list_t T) (i : U32) (ret0 : (T × T)) :
   Result ((list_t T) × (list_t T))
   :=
-  list_nth_mut_loop_pair_merge_loop_back T ls0 ls1 i ret0
+  do
+    let p ⟵ list_nth_mut_loop_pair_merge_loop_back T ls0 ls1 i ret0
+    let (l, l0) := p
+    Result.ret (l, l0)
 
 /- [loops::list_nth_shared_loop_pair_merge] -/
 def list_nth_shared_loop_pair_merge_loop_fwd
   (T : Type) (ls0 : list_t T) (ls1 : list_t T) (i : U32) : (Result (T × T)) :=
-  match h: ls0 with
+  match 𝒽: ls0 with
   | list_t.Cons x0 tl0 =>
-    match h: ls1 with
+    match 𝒽: ls1 with
     | list_t.Cons x1 tl1 =>
-      if h: i = (U32.ofInt 0 (by intlit))
+      if 𝒽: i = (U32.ofInt 0 (by intlit))
       then Result.ret (x0, x1)
       else
         do
-          let i0 ← i - (U32.ofInt 1 (by intlit))
-          list_nth_shared_loop_pair_merge_loop_fwd T tl0 tl1 i0
+          let i0 ⟵ i - (U32.ofInt 1 (by intlit))
+          let p ⟵ list_nth_shared_loop_pair_merge_loop_fwd T tl0 tl1 i0
+          Result.ret p
     | list_t.Nil => Result.fail Error.panic
   | list_t.Nil => Result.fail Error.panic
 termination_by list_nth_shared_loop_pair_merge_loop_fwd ls0 ls1 i =>
@@ -485,21 +539,24 @@ decreasing_by list_nth_shared_loop_pair_merge_loop_decreases ls0 ls1 i
 /- [loops::list_nth_shared_loop_pair_merge] -/
 def list_nth_shared_loop_pair_merge_fwd
   (T : Type) (ls0 : list_t T) (ls1 : list_t T) (i : U32) : Result (T × T) :=
-  list_nth_shared_loop_pair_merge_loop_fwd T ls0 ls1 i
+  do
+    let p ⟵ list_nth_shared_loop_pair_merge_loop_fwd T ls0 ls1 i
+    Result.ret p
 
 /- [loops::list_nth_mut_shared_loop_pair] -/
 def list_nth_mut_shared_loop_pair_loop_fwd
   (T : Type) (ls0 : list_t T) (ls1 : list_t T) (i : U32) : (Result (T × T)) :=
-  match h: ls0 with
+  match 𝒽: ls0 with
   | list_t.Cons x0 tl0 =>
-    match h: ls1 with
+    match 𝒽: ls1 with
     | list_t.Cons x1 tl1 =>
-      if h: i = (U32.ofInt 0 (by intlit))
+      if 𝒽: i = (U32.ofInt 0 (by intlit))
       then Result.ret (x0, x1)
       else
         do
-          let i0 ← i - (U32.ofInt 1 (by intlit))
-          list_nth_mut_shared_loop_pair_loop_fwd T tl0 tl1 i0
+          let i0 ⟵ i - (U32.ofInt 1 (by intlit))
+          let p ⟵ list_nth_mut_shared_loop_pair_loop_fwd T tl0 tl1 i0
+          Result.ret p
     | list_t.Nil => Result.fail Error.panic
   | list_t.Nil => Result.fail Error.panic
 termination_by list_nth_mut_shared_loop_pair_loop_fwd ls0 ls1 i =>
@@ -509,23 +566,25 @@ decreasing_by list_nth_mut_shared_loop_pair_loop_decreases ls0 ls1 i
 /- [loops::list_nth_mut_shared_loop_pair] -/
 def list_nth_mut_shared_loop_pair_fwd
   (T : Type) (ls0 : list_t T) (ls1 : list_t T) (i : U32) : Result (T × T) :=
-  list_nth_mut_shared_loop_pair_loop_fwd T ls0 ls1 i
+  do
+    let p ⟵ list_nth_mut_shared_loop_pair_loop_fwd T ls0 ls1 i
+    Result.ret p
 
 /- [loops::list_nth_mut_shared_loop_pair] -/
 def list_nth_mut_shared_loop_pair_loop_back
   (T : Type) (ls0 : list_t T) (ls1 : list_t T) (i : U32) (ret0 : T) :
   (Result (list_t T))
   :=
-  match h: ls0 with
+  match 𝒽: ls0 with
   | list_t.Cons x0 tl0 =>
-    match h: ls1 with
+    match 𝒽: ls1 with
     | list_t.Cons x1 tl1 =>
-      if h: i = (U32.ofInt 0 (by intlit))
+      if 𝒽: i = (U32.ofInt 0 (by intlit))
       then Result.ret (list_t.Cons ret0 tl0)
       else
         do
-          let i0 ← i - (U32.ofInt 1 (by intlit))
-          let tl00 ←
+          let i0 ⟵ i - (U32.ofInt 1 (by intlit))
+          let tl00 ⟵
             list_nth_mut_shared_loop_pair_loop_back T tl0 tl1 i0 ret0
           Result.ret (list_t.Cons x0 tl00)
     | list_t.Nil => Result.fail Error.panic
@@ -539,21 +598,24 @@ def list_nth_mut_shared_loop_pair_back
   (T : Type) (ls0 : list_t T) (ls1 : list_t T) (i : U32) (ret0 : T) :
   Result (list_t T)
   :=
-  list_nth_mut_shared_loop_pair_loop_back T ls0 ls1 i ret0
+  do
+    let l ⟵ list_nth_mut_shared_loop_pair_loop_back T ls0 ls1 i ret0
+    Result.ret l
 
 /- [loops::list_nth_mut_shared_loop_pair_merge] -/
 def list_nth_mut_shared_loop_pair_merge_loop_fwd
   (T : Type) (ls0 : list_t T) (ls1 : list_t T) (i : U32) : (Result (T × T)) :=
-  match h: ls0 with
+  match 𝒽: ls0 with
   | list_t.Cons x0 tl0 =>
-    match h: ls1 with
+    match 𝒽: ls1 with
     | list_t.Cons x1 tl1 =>
-      if h: i = (U32.ofInt 0 (by intlit))
+      if 𝒽: i = (U32.ofInt 0 (by intlit))
       then Result.ret (x0, x1)
       else
         do
-          let i0 ← i - (U32.ofInt 1 (by intlit))
-          list_nth_mut_shared_loop_pair_merge_loop_fwd T tl0 tl1 i0
+          let i0 ⟵ i - (U32.ofInt 1 (by intlit))
+          let p ⟵ list_nth_mut_shared_loop_pair_merge_loop_fwd T tl0 tl1 i0
+          Result.ret p
     | list_t.Nil => Result.fail Error.panic
   | list_t.Nil => Result.fail Error.panic
 termination_by list_nth_mut_shared_loop_pair_merge_loop_fwd ls0 ls1 i =>
@@ -563,23 +625,25 @@ decreasing_by list_nth_mut_shared_loop_pair_merge_loop_decreases ls0 ls1 i
 /- [loops::list_nth_mut_shared_loop_pair_merge] -/
 def list_nth_mut_shared_loop_pair_merge_fwd
   (T : Type) (ls0 : list_t T) (ls1 : list_t T) (i : U32) : Result (T × T) :=
-  list_nth_mut_shared_loop_pair_merge_loop_fwd T ls0 ls1 i
+  do
+    let p ⟵ list_nth_mut_shared_loop_pair_merge_loop_fwd T ls0 ls1 i
+    Result.ret p
 
 /- [loops::list_nth_mut_shared_loop_pair_merge] -/
 def list_nth_mut_shared_loop_pair_merge_loop_back
   (T : Type) (ls0 : list_t T) (ls1 : list_t T) (i : U32) (ret0 : T) :
   (Result (list_t T))
   :=
-  match h: ls0 with
+  match 𝒽: ls0 with
   | list_t.Cons x0 tl0 =>
-    match h: ls1 with
+    match 𝒽: ls1 with
     | list_t.Cons x1 tl1 =>
-      if h: i = (U32.ofInt 0 (by intlit))
+      if 𝒽: i = (U32.ofInt 0 (by intlit))
       then Result.ret (list_t.Cons ret0 tl0)
       else
         do
-          let i0 ← i - (U32.ofInt 1 (by intlit))
-          let tl00 ←
+          let i0 ⟵ i - (U32.ofInt 1 (by intlit))
+          let tl00 ⟵
             list_nth_mut_shared_loop_pair_merge_loop_back T tl0 tl1 i0 ret0
           Result.ret (list_t.Cons x0 tl00)
     | list_t.Nil => Result.fail Error.panic
@@ -593,21 +657,24 @@ def list_nth_mut_shared_loop_pair_merge_back
   (T : Type) (ls0 : list_t T) (ls1 : list_t T) (i : U32) (ret0 : T) :
   Result (list_t T)
   :=
-  list_nth_mut_shared_loop_pair_merge_loop_back T ls0 ls1 i ret0
+  do
+    let l ⟵ list_nth_mut_shared_loop_pair_merge_loop_back T ls0 ls1 i ret0
+    Result.ret l
 
 /- [loops::list_nth_shared_mut_loop_pair] -/
 def list_nth_shared_mut_loop_pair_loop_fwd
   (T : Type) (ls0 : list_t T) (ls1 : list_t T) (i : U32) : (Result (T × T)) :=
-  match h: ls0 with
+  match 𝒽: ls0 with
   | list_t.Cons x0 tl0 =>
-    match h: ls1 with
+    match 𝒽: ls1 with
     | list_t.Cons x1 tl1 =>
-      if h: i = (U32.ofInt 0 (by intlit))
+      if 𝒽: i = (U32.ofInt 0 (by intlit))
       then Result.ret (x0, x1)
       else
         do
-          let i0 ← i - (U32.ofInt 1 (by intlit))
-          list_nth_shared_mut_loop_pair_loop_fwd T tl0 tl1 i0
+          let i0 ⟵ i - (U32.ofInt 1 (by intlit))
+          let p ⟵ list_nth_shared_mut_loop_pair_loop_fwd T tl0 tl1 i0
+          Result.ret p
     | list_t.Nil => Result.fail Error.panic
   | list_t.Nil => Result.fail Error.panic
 termination_by list_nth_shared_mut_loop_pair_loop_fwd ls0 ls1 i =>
@@ -617,23 +684,25 @@ decreasing_by list_nth_shared_mut_loop_pair_loop_decreases ls0 ls1 i
 /- [loops::list_nth_shared_mut_loop_pair] -/
 def list_nth_shared_mut_loop_pair_fwd
   (T : Type) (ls0 : list_t T) (ls1 : list_t T) (i : U32) : Result (T × T) :=
-  list_nth_shared_mut_loop_pair_loop_fwd T ls0 ls1 i
+  do
+    let p ⟵ list_nth_shared_mut_loop_pair_loop_fwd T ls0 ls1 i
+    Result.ret p
 
 /- [loops::list_nth_shared_mut_loop_pair] -/
 def list_nth_shared_mut_loop_pair_loop_back
   (T : Type) (ls0 : list_t T) (ls1 : list_t T) (i : U32) (ret0 : T) :
   (Result (list_t T))
   :=
-  match h: ls0 with
+  match 𝒽: ls0 with
   | list_t.Cons x0 tl0 =>
-    match h: ls1 with
+    match 𝒽: ls1 with
     | list_t.Cons x1 tl1 =>
-      if h: i = (U32.ofInt 0 (by intlit))
+      if 𝒽: i = (U32.ofInt 0 (by intlit))
       then Result.ret (list_t.Cons ret0 tl1)
       else
         do
-          let i0 ← i - (U32.ofInt 1 (by intlit))
-          let tl10 ←
+          let i0 ⟵ i - (U32.ofInt 1 (by intlit))
+          let tl10 ⟵
             list_nth_shared_mut_loop_pair_loop_back T tl0 tl1 i0 ret0
           Result.ret (list_t.Cons x1 tl10)
     | list_t.Nil => Result.fail Error.panic
@@ -647,21 +716,24 @@ def list_nth_shared_mut_loop_pair_back
   (T : Type) (ls0 : list_t T) (ls1 : list_t T) (i : U32) (ret0 : T) :
   Result (list_t T)
   :=
-  list_nth_shared_mut_loop_pair_loop_back T ls0 ls1 i ret0
+  do
+    let l ⟵ list_nth_shared_mut_loop_pair_loop_back T ls0 ls1 i ret0
+    Result.ret l
 
 /- [loops::list_nth_shared_mut_loop_pair_merge] -/
 def list_nth_shared_mut_loop_pair_merge_loop_fwd
   (T : Type) (ls0 : list_t T) (ls1 : list_t T) (i : U32) : (Result (T × T)) :=
-  match h: ls0 with
+  match 𝒽: ls0 with
   | list_t.Cons x0 tl0 =>
-    match h: ls1 with
+    match 𝒽: ls1 with
     | list_t.Cons x1 tl1 =>
-      if h: i = (U32.ofInt 0 (by intlit))
+      if 𝒽: i = (U32.ofInt 0 (by intlit))
       then Result.ret (x0, x1)
       else
         do
-          let i0 ← i - (U32.ofInt 1 (by intlit))
-          list_nth_shared_mut_loop_pair_merge_loop_fwd T tl0 tl1 i0
+          let i0 ⟵ i - (U32.ofInt 1 (by intlit))
+          let p ⟵ list_nth_shared_mut_loop_pair_merge_loop_fwd T tl0 tl1 i0
+          Result.ret p
     | list_t.Nil => Result.fail Error.panic
   | list_t.Nil => Result.fail Error.panic
 termination_by list_nth_shared_mut_loop_pair_merge_loop_fwd ls0 ls1 i =>
@@ -671,23 +743,25 @@ decreasing_by list_nth_shared_mut_loop_pair_merge_loop_decreases ls0 ls1 i
 /- [loops::list_nth_shared_mut_loop_pair_merge] -/
 def list_nth_shared_mut_loop_pair_merge_fwd
   (T : Type) (ls0 : list_t T) (ls1 : list_t T) (i : U32) : Result (T × T) :=
-  list_nth_shared_mut_loop_pair_merge_loop_fwd T ls0 ls1 i
+  do
+    let p ⟵ list_nth_shared_mut_loop_pair_merge_loop_fwd T ls0 ls1 i
+    Result.ret p
 
 /- [loops::list_nth_shared_mut_loop_pair_merge] -/
 def list_nth_shared_mut_loop_pair_merge_loop_back
   (T : Type) (ls0 : list_t T) (ls1 : list_t T) (i : U32) (ret0 : T) :
   (Result (list_t T))
   :=
-  match h: ls0 with
+  match 𝒽: ls0 with
   | list_t.Cons x0 tl0 =>
-    match h: ls1 with
+    match 𝒽: ls1 with
     | list_t.Cons x1 tl1 =>
-      if h: i = (U32.ofInt 0 (by intlit))
+      if 𝒽: i = (U32.ofInt 0 (by intlit))
       then Result.ret (list_t.Cons ret0 tl1)
       else
         do
-          let i0 ← i - (U32.ofInt 1 (by intlit))
-          let tl10 ←
+          let i0 ⟵ i - (U32.ofInt 1 (by intlit))
+          let tl10 ⟵
             list_nth_shared_mut_loop_pair_merge_loop_back T tl0 tl1 i0 ret0
           Result.ret (list_t.Cons x1 tl10)
     | list_t.Nil => Result.fail Error.panic
@@ -701,5 +775,7 @@ def list_nth_shared_mut_loop_pair_merge_back
   (T : Type) (ls0 : list_t T) (ls1 : list_t T) (i : U32) (ret0 : T) :
   Result (list_t T)
   :=
-  list_nth_shared_mut_loop_pair_merge_loop_back T ls0 ls1 i ret0
+  do
+    let l ⟵ list_nth_shared_mut_loop_pair_merge_loop_back T ls0 ls1 i ret0
+    Result.ret l
 
