tests/lean/misc-paper/Paper.lean
@@ -9,8 +9,8 @@ def ref_incr_fwd_back (x : I32) : Result I32 :=
 /- [paper::test_incr] -/
 def test_incr_fwd : Result Unit :=
   do
-    let x ← ref_incr_fwd_back (I32.ofInt 0 (by intlit))
-    if h: not (x = (I32.ofInt 1 (by intlit)))
+    let x ⟵ ref_incr_fwd_back (I32.ofInt 0 (by intlit))
+    if 𝒽: not (x = (I32.ofInt 1 (by intlit)))
     then Result.fail Error.panic
     else Result.ret ()
 
@@ -19,34 +19,34 @@ def test_incr_fwd : Result Unit :=
 
 /- [paper::choose] -/
 def choose_fwd (T : Type) (b : Bool) (x : T) (y : T) : Result T :=
-  if h: b
+  if 𝒽: b
   then Result.ret x
   else Result.ret y
 
 /- [paper::choose] -/
 def choose_back
   (T : Type) (b : Bool) (x : T) (y : T) (ret0 : T) : Result (T × T) :=
-  if h: b
+  if 𝒽: b
   then Result.ret (ret0, y)
   else Result.ret (x, ret0)
 
 /- [paper::test_choose] -/
 def test_choose_fwd : Result Unit :=
   do
-    let z ←
+    let z ⟵
       choose_fwd I32 true (I32.ofInt 0 (by intlit)) (I32.ofInt 0 (by intlit))
-    let z0 ← z + (I32.ofInt 1 (by intlit))
-    if h: not (z0 = (I32.ofInt 1 (by intlit)))
+    let z0 ⟵ z + (I32.ofInt 1 (by intlit))
+    if 𝒽: not (z0 = (I32.ofInt 1 (by intlit)))
     then Result.fail Error.panic
     else
       do
-        let (x, y) ←
+        let (x, y) ⟵
           choose_back I32 true (I32.ofInt 0 (by intlit))
             (I32.ofInt 0 (by intlit)) z0
-        if h: not (x = (I32.ofInt 1 (by intlit)))
+        if 𝒽: not (x = (I32.ofInt 1 (by intlit)))
         then Result.fail Error.panic
         else
-          if h: not (y = (I32.ofInt 0 (by intlit)))
+          if 𝒽: not (y = (I32.ofInt 0 (by intlit)))
           then Result.fail Error.panic
           else Result.ret ()
 
@@ -60,34 +60,36 @@ inductive list_t (T : Type) :=
 
 /- [paper::list_nth_mut] -/
 def list_nth_mut_fwd (T : Type) (l : list_t T) (i : U32) : Result T :=
-  match h: l with
+  match 𝒽: l with
   | list_t.Cons x tl =>
-    if h: i = (U32.ofInt 0 (by intlit))
+    if 𝒽: i = (U32.ofInt 0 (by intlit))
     then Result.ret x
-    else do
-           let i0 ← i - (U32.ofInt 1 (by intlit))
-           list_nth_mut_fwd T tl i0
+    else
+      do
+        let i0 ⟵ i - (U32.ofInt 1 (by intlit))
+        let t ⟵ list_nth_mut_fwd T tl i0
+        Result.ret t
   | list_t.Nil => Result.fail Error.panic
 
 /- [paper::list_nth_mut] -/
 def list_nth_mut_back
   (T : Type) (l : list_t T) (i : U32) (ret0 : T) : Result (list_t T) :=
-  match h: l with
+  match 𝒽: l with
   | list_t.Cons x tl =>
-    if h: i = (U32.ofInt 0 (by intlit))
+    if 𝒽: i = (U32.ofInt 0 (by intlit))
     then Result.ret (list_t.Cons ret0 tl)
     else
       do
-        let i0 ← i - (U32.ofInt 1 (by intlit))
-        let tl0 ← list_nth_mut_back T tl i0 ret0
+        let i0 ⟵ i - (U32.ofInt 1 (by intlit))
+        let tl0 ⟵ list_nth_mut_back T tl i0 ret0
         Result.ret (list_t.Cons x tl0)
   | list_t.Nil => Result.fail Error.panic
 
 /- [paper::sum] -/
 def sum_fwd (l : list_t I32) : Result I32 :=
-  match h: l with
+  match 𝒽: l with
   | list_t.Cons x tl => do
-                          let i ← sum_fwd tl
+                          let i ⟵ sum_fwd tl
                           x + i
   | list_t.Nil => Result.ret (I32.ofInt 0 (by intlit))
 
@@ -97,15 +99,15 @@ def test_nth_fwd : Result Unit :=
     let l := list_t.Nil
     let l0 := list_t.Cons (I32.ofInt 3 (by intlit)) l
     let l1 := list_t.Cons (I32.ofInt 2 (by intlit)) l0
-    let x ←
+    let x ⟵
       list_nth_mut_fwd I32 (list_t.Cons (I32.ofInt 1 (by intlit)) l1)
         (U32.ofInt 2 (by intlit))
-    let x0 ← x + (I32.ofInt 1 (by intlit))
-    let l2 ←
+    let x0 ⟵ x + (I32.ofInt 1 (by intlit))
+    let l2 ⟵
       list_nth_mut_back I32 (list_t.Cons (I32.ofInt 1 (by intlit)) l1)
         (U32.ofInt 2 (by intlit)) x0
-    let i ← sum_fwd l2
-    if h: not (i = (I32.ofInt 7 (by intlit)))
+    let i ⟵ sum_fwd l2
+    if 𝒽: not (i = (I32.ofInt 7 (by intlit)))
     then Result.fail Error.panic
     else Result.ret ()
 
@@ -116,8 +118,8 @@ def test_nth_fwd : Result Unit :=
 def call_choose_fwd (p : (U32 × U32)) : Result U32 :=
   do
     let (px, py) := p
-    let pz ← choose_fwd U32 true px py
-    let pz0 ← pz + (U32.ofInt 1 (by intlit))
-    let (px0, _) ← choose_back U32 true px py pz0
+    let pz ⟵ choose_fwd U32 true px py
+    let pz0 ⟵ pz + (U32.ofInt 1 (by intlit))
+    let (px0, _) ⟵ choose_back U32 true px py pz0
     Result.ret px0
 
