tests/lean/misc-polonius_list/PoloniusList.lean
@@ -9,23 +9,25 @@ inductive list_t (T : Type) :=
 
 /- [polonius_list::get_list_at_x] -/
 def get_list_at_x_fwd (ls : list_t U32) (x : U32) : Result (list_t U32) :=
-  match h: ls with
+  match 𝒽: ls with
   | list_t.Cons hd tl =>
-    if h: hd = x
+    if 𝒽: hd = x
     then Result.ret (list_t.Cons hd tl)
-    else get_list_at_x_fwd tl x
+    else do
+           let l ⟵ get_list_at_x_fwd tl x
+           Result.ret l
   | list_t.Nil => Result.ret list_t.Nil
 
 /- [polonius_list::get_list_at_x] -/
 def get_list_at_x_back
   (ls : list_t U32) (x : U32) (ret0 : list_t U32) : Result (list_t U32) :=
-  match h: ls with
+  match 𝒽: ls with
   | list_t.Cons hd tl =>
-    if h: hd = x
+    if 𝒽: hd = x
     then Result.ret ret0
     else
       do
-        let tl0 ← get_list_at_x_back tl x ret0
+        let tl0 ⟵ get_list_at_x_back tl x ret0
         Result.ret (list_t.Cons hd tl0)
   | list_t.Nil => Result.ret ret0
 
